Parser semi-working, hello James

Experiments/ProofChecking/RangeArray.lean
@@ -8,7 +8,9 @@ Carnegie Mellon University
 
 -/
 
-import Experiments.ProofChecking.CArray
+-- It appears that we don't need to use these
+--import Experiments.ProofChecking.CArray
+import Experiments.ProofChecking.Array
 
 import Mathlib.Data.Nat.Basic
 import Mathlib.Data.Array.Basic
@@ -17,69 +19,134 @@ import Mathlib.Tactic
 import LeanSAT.Upstream.ToStd
 import LeanSAT.Upstream.ToMathlib
 
+import LeanSAT.Data.Cnf
+import LeanSAT.Data.ICnf
+import LeanSAT.Model.PropFun
+
+import LeanColls
+
+open LeanColls
+
+namespace Fin
+
+def foldRangeM {β : Type v} {m : Type v → Type w} [Monad m]
+    {n : Nat} (f : Fin n → β → m β) (init : β) (s e : Fin n) : m β :=
+  let rec loop (i : Fin n) (b : β) : m β := do
+    if h : i < e then
+      loop ⟨i.val + 1, lt_of_le_of_lt (Nat.succ_le_of_lt h) e.isLt⟩ (← f ⟨i, by exact lt_trans h e.isLt⟩ b)
+    else
+      pure b
+  termination_by e.val - i.val
+  loop s init
+
+def foldRange {β : Type v} (f : Fin n → β → β) (init : β) (s e : Fin n) : β :=
+  Id.run <| foldRangeM f init s e
+
+@[simp]
+theorem foldRangeM_eq {β : Type v} {m : Type v → Type w} [Monad m]
+    (f : Fin n → β → m β) (init : β) (s : Fin n) :
+    foldRangeM f init s s = return init := by
+  simp [foldRange, foldRangeM, foldRangeM.loop]
+
+theorem foldRangeM_lt {β : Type v} {m : Type v → Type w} [Monad m]
+    (f : Fin n → β → m β) (init : β) (s e : Fin n) (h : s < e) :
+    foldRangeM f init s e = do
+      { foldRangeM f (← f s init) ⟨s.val + 1, lt_of_le_of_lt (Nat.succ_le_of_lt h) e.isLt⟩ e } := by
+  simp [foldRange, foldRangeM]
+  rw [foldRangeM.loop]
+  simp [h]
+
+theorem foldRangeM_gt {β : Type v} {m : Type v → Type w} [Monad m]
+    (f : Fin n → β → m β) (init : β) (s e : Fin n) (h : e < s) :
+    foldRangeM f init s e = return init := by
+  simp [foldRange, foldRangeM]
+  rw [foldRangeM.loop]
+  simp [h]
+  exact fun hcon => absurd (le_of_lt hcon) (not_le_of_gt h)
+
+@[simp]
+theorem foldRange_eq {β : Type v} (f : Fin n → β → β) (init : β) (s : Fin n) :
+    foldRange f init s s = init := by
+  simp [foldRange, foldRangeM, Id.run, foldRangeM.loop]
+
+theorem foldRange_lt {β : Type v} (f : Fin n → β → β) (init : β) (s e : Fin n) (h : s < e) :
+    foldRange f init s e = foldRange f (f s init) ⟨s.val + 1, lt_of_le_of_lt (Nat.succ_le_of_lt h) e.isLt⟩ e := by
+  simp [foldRange, foldRangeM]
+  rw [foldRangeM.loop]
+  simp [h]
+
+theorem foldRange_gt {β : Type v} (f : Fin n → β → β) (init : β) (s e : Fin n) (h : e < s) :
+    foldRange f init s e = init := by
+  simp [foldRange, foldRangeM, Id.run]
+  rw [foldRangeM.loop]
+  simp [h]
+  exact fun hcon => absurd (le_of_lt hcon) (not_le_of_gt h)
+
+end Fin
+
 /-
   A structure with a single pool of data in an array, and a system for marking
   contiguous regions of that pool into pieces. Also handles deletions.
 -/
 structure RangeArray (α : Type _) where
-  data : CArray α
-  indexes : CArray Nat
-  deleted : CArray Bool
+  data : Array α
+  indexes : Array Nat
+  deleted : Array Bool
   deletedSize : Nat /-- Counts the total size of the data array that has been deleted. -/
 
   /- We want every index in the RangeArray to point "into" data in bounds. However,
      the clearing property makes it so that the data beyond the lsize limit in
      indexes might be larger than data's logical size (lsize). So we separate out
      the hypothesis that everything in the logical data of indexes is in bounds. -/
-  h_indexes : ∀ (i : Fin indexes.size), (indexes.get i) < data.size + 1
-  h_sizes : indexes.size = deleted.size ∧ indexes.size > 0
+  h_indexes_size_pos : indexes.size > 0
+  h_indexes : ∀ (i : Fin indexes.size), (indexes.get i) ≤ data.size
+  h_sizes_eq : indexes.size = deleted.size
 
 namespace RangeArray
 
-open Nat CArray
+open Nat Array
 
 variable {α : Type u} (A : RangeArray α) (v : α)
 
 def mkRangeArray (n : Nat) (v : α) : RangeArray α := {
-  data := CArray.mkCArray n v
-  indexes := CArray.singleton 0
-  deleted := CArray.singleton true
+  data := Array.mkArray n v
+  indexes := Array.singleton 0
+  deleted := Array.singleton true
   deletedSize := 0
-  h_indexes := by
-    intro i
-    simp [size_mkCArray, CArray.singleton, CArray.get]
-    exact succ_pos _
-  h_sizes := by simp
+  h_indexes := by simp; intro; exact Nat.zero_le _
+  h_indexes_size_pos := by simp
+  h_sizes_eq := by simp
 }
 
 def empty : RangeArray α := {
-  data := CArray.empty
-  indexes := CArray.singleton 0
-  deleted := CArray.singleton true
+  data := Array.empty
+  indexes := Array.singleton 0
+  deleted := Array.singleton true
   deletedSize := 0
-  h_indexes := by
-    intro i
-    simp [size_mkCArray, CArray.singleton, CArray.get]
-    exact succ_pos _
-  h_sizes := by simp
+  h_indexes := by simp; intro; exact Nat.zero_le _
+  h_indexes_size_pos := by simp
+  h_sizes_eq := by simp
 }
 
-/-- The (logical) size of the underlying data array. -/
-def size : Nat := A.data.size
+/-- The (logical) size of the number of indexes (including unfinished backs). -/
+abbrev size : Nat := A.indexes.size
 
-/-- The (logical) number of partitions in the underlying data array
-    Excludes 1 due to allowing an "extra" element on the end.  -/
-def numPartitions : Nat := A.indexes.size - 1
+/-- The (logical) size of the underlying data array. -/
+abbrev dsize : Nat := A.data.size
+
+/-- The (logical) number of times `cap` has been called. -/
+abbrev caps : Nat := A.indexes.size - 1
 
 /-- Pushes an element of data onto the back of the data array.
-    By default, new "partitions" are deleted until `cap` is called. -/
+    By default, new "partitions" are considered deleted until `push` is called. -/
 def push : RangeArray α := { A with
   data := A.data.push v
   deleted := A.deleted.setBack false
   h_indexes := by
+    simp
     intro i
-    rw [size_push]
-    exact lt_succ_of_lt (A.h_indexes i)
+    exact le_trans (A.h_indexes i) (Nat.le_succ _)
+  h_sizes_eq := by simp [A.h_sizes_eq]
 }
 
 -- Caps off the current section (by adding the start of the next section)
@@ -88,38 +155,233 @@ def cap : RangeArray α := { A with
   indexes := A.indexes.push A.data.size
   deleted := A.deleted.push true
   h_indexes := by
-    intro i
-    rcases i with ⟨i, hi⟩
-    rw [size_push] at hi
-    rcases Order.lt_succ_iff_eq_or_lt.mp hi with (rfl | hi)
+    rintro ⟨i, hi⟩
+    simp at hi ⊢
+    rcases eq_or_lt_of_le (le_of_lt_succ hi) with (rfl | hi)
     · simp
-    · rw [get_push_lt A.indexes (A.data.size) ⟨i, hi⟩]
-      exact A.h_indexes _
-  h_sizes := by simp [A.h_sizes]
+    · simp [get_push, hi]
+      exact A.h_indexes ⟨i, hi⟩
+  h_indexes_size_pos := by simp
+  h_sizes_eq := by simp [A.h_sizes_eq]
 }
 
 -- Calls cap until the desired number of caps is reached
-def capUntil (desiredNumCaps : Nat) : RangeArray α :=
+def capUntil (desiredCaps : Nat) : RangeArray α :=
   let rec loop (j : Nat) (A' : RangeArray α) : RangeArray α :=
     match j with
     | 0     => A'
     | j + 1 => loop j (A'.cap)
-  loop (desiredNumCaps - A.numPartitions) A
+  loop (desiredCaps - A.caps) A
 
-def clear : RangeArray α := { A with
-  data := A.data.clear
-  indexes := A.indexes.clear.push 0
-  deleted := A.deleted.clear.push true
-  h_indexes := by
-    intro i
+def index (i : Fin A.size) : Nat := A.indexes.get i
+
+/-- Gets the size of the range under the provided index. -/
+def rsize (i : Fin A.size) : Nat :=
+  if hi : i.val + 1 < A.size then
+    A.index ⟨i.val + 1, hi⟩ - A.index i
+  else
+    A.dsize - A.index i
+
+theorem rsize_lt_size (i : Fin A.size) : A.rsize i ≤ A.dsize - A.index i := by
+  simp [index, rsize]
+  by_cases h_index : i.val + 1 < A.size <;> simp [h_index]
+  rw [Nat.sub_add_cancel]
+  exact A.h_indexes ⟨i.val + 1, h_index⟩
+  exact A.h_indexes i
+
+def get (i : Fin A.size) (j : Fin (A.rsize i)) : α :=
+  A.data.get ⟨A.index i, by
     rcases i with ⟨i, hi⟩
-    simp at hi
-    have := get_push_eq (A.indexes.clear) 0
-    rw [size_clear] at this
-    aesop
-  h_sizes := by simp
+    rcases j with ⟨j, hj⟩
+    have := A.h_indexes ⟨i, hi⟩
+    rcases eq_or_lt_of_le this with (hi_eq | hi_lt)
+    · have h : A.dsize - A.index ⟨i, hi⟩ = 0 := by
+        exact (Nat.sub_eq_iff_eq_add' this).mpr (id hi_eq.symm)
+      have := rsize_lt_size _ ⟨i, hi⟩
+      rw [h, le_zero] at this
+      rw [this] at hj
+      contradiction
+    · exact hi_lt⟩
+
+def delete (i : Fin A.size) : RangeArray α := { A with
+  deleted := A.deleted.set ⟨i, by rw [← A.h_sizes_eq]; exact i.isLt⟩ true
+  deletedSize := A.deletedSize + A.rsize i
+  h_sizes_eq := by simp [A.h_sizes_eq]
 }
 
+def isDeleted (i : Fin A.size) : Bool := A.deleted.get ⟨i, by rw [← A.h_sizes_eq]; exact i.isLt⟩
+
+@[simp] theorem size_empty : (empty : RangeArray α).size = 1 := by simp [empty, size]
+@[simp] theorem dsize_empty : (empty : RangeArray α).dsize = 0 := by simp [empty, dsize]; rfl
+@[simp] theorem rsize_empty : (empty : RangeArray α).rsize ⟨0, by simp⟩ = 0 := by simp [empty]; rfl
+@[simp] theorem size_push : (A.push v).size = A.size := by simp [push, size]
+@[simp] theorem dsize_push : (A.push v).dsize = A.dsize + 1 := by simp [push, dsize]
+
+@[simp]
+theorem rsize_push (i : Fin A.size) : (A.push v).rsize i =
+    if i.val + 1 = A.size then A.rsize i + 1 else A.rsize i := by
+  simp [push, rsize]
+  rcases i with ⟨i, hi⟩
+  by_cases h_index : i + 1 < A.size
+  · simp [h_index, Nat.ne_of_lt h_index]; rfl
+  · simp [h_index]
+    simp at h_index
+    simp [le_antisymm h_index (succ_le_of_lt hi), index]
+    rw [Nat.sub_add_comm]
+    exact A.h_indexes _
+
+@[simp] theorem size_cap : (A.cap).size = A.size + 1 := by simp [cap, size]
+@[simp] theorem dsize_cap : (A.cap).dsize = A.dsize := by simp [cap, dsize]
+
+@[simp]
+theorem rsize_cap (i : Fin A.size) : (A.cap).rsize ⟨i.val, by rw [size_cap]; exact lt_succ_of_lt i.isLt⟩ = A.rsize i := by
+  simp [cap, rsize, index]; sorry
+
+@[simp] theorem size_delete (i : Fin A.size) : (A.delete i).size = A.size := by simp [delete, size]
+@[simp] theorem dsize_delete (i : Fin A.size) : (A.delete i).dsize = A.dsize := by simp [delete, dsize]
+
+@[simp]
+theorem rsize_delete (i j : Fin A.size) : (A.delete i).rsize j =
+    if i.val = j.val then 0 else A.rsize j := by
+  simp [delete, rsize]; sorry
+
+def zeroFin : Fin A.size := ⟨0, A.h_indexes_size_pos⟩
+def predFin : Fin A.size := ⟨A.size - 1, by
+    match hA' : A.size with
+    | 0 => have hA := A.h_indexes_size_pos; simp [hA'] at hA; | n + 1 => simp⟩
+
+@[inline, specialize]
+def foldlM_index {β : Type v} {m : Type v → Type w} [Monad m] (f : β → α → m β)
+    (init : β) (A : RangeArray α) (i : Fin A.size) : m β :=
+  A.data.foldlM f init (A.index i) (A.index i + A.rsize i)
+
+@[inline]
+def foldl_index {β : Type v} (f : β → α → β)
+    (init : β) (A : RangeArray α) (i : Fin A.size) : β :=
+  Id.run <| A.foldlM_index f init i
+
+@[simp]
+theorem foldlM_index_empty {β : Type v} {m : Type v → Type w} [Monad m]
+    (f : β → α → m β) (init : β) (i : Fin empty.size) :
+      (empty : RangeArray α).foldlM_index f init i = return init := by
+  simp [foldlM_index, empty, foldlM]
+  rcases i with ⟨i, hi⟩
+  simp at hi
+  subst hi
+  simp
+  sorry
+
+@[simp]
+theorem foldl_index_empty {β : Type v} (f : β → α → β) (init : β) (i : Fin empty.size) :
+      (empty : RangeArray α).foldl_index f init i = init := by
+  simp [foldl_index, empty, foldlM_index_empty]
+  sorry
+
+theorem foldl_index_push_lt {β : Type v} (f : β → α → β) (init : β) (i : Fin A.size) (h : i.val + 1 < A.size) :
+    (A.push v).foldl_index f init i = A.foldl_index f init i := by
+  simp [foldl_index, push, foldlM_index]
+  sorry
+
+theorem foldl_index_push_eq {β : Type v} (f : β → α → β) (init : β) (i : Fin A.size) (h : i.val + 1 = A.size) :
+    (A.push v).foldl_index f init i = f init v := by
+  simp [foldl_index, push, foldlM_index]
+  sorry
+
+/-
+@[inline, specialize]
+def foldlM {α : Type u} {β : Type v} {γ : Type w} {m₁ : Type v → Type w} {m₂ : Type w → Type x}
+    [Monad m₁] [Monad m₂] (f_inner : β → α → m₁ β) (f_outer : γ → β → m₂ γ)
+    (init_inner : β) (init_outer : γ) (A : RangeArray α) (start stop : Fin A.size) : m₂ γ := -/
+
+@[inline, specialize]
+def foldlM {α : Type u} {β : Type v} {m : Type v → Type w}
+    [Monad m] (f_inner : β → α → m β) (f_outer : β → β → m β)
+    (init_inner init_outer : β) (A : RangeArray α)
+    (start : Fin A.size := A.zeroFin)
+    (stop : Fin A.size := A.predFin) : m β :=
+  Fin.foldRangeM (fun i b => do
+    if !A.isDeleted i then
+      f_outer b (← A.foldlM_index f_inner init_inner i)
+    else
+      return b) init_outer start stop
+
+@[inline]
+def foldl {α : Type u} {β : Type v} (f_inner : β → α → β) (f_outer : β → β → β)
+    (init_inner init_outer : β) (A : RangeArray α)
+      (start : Fin A.size := A.zeroFin)
+      (stop : Fin A.size := A.predFin) : β :=
+  Fin.foldRange (fun i b => f_outer b (A.foldl_index f_inner init_inner i)) init_outer start stop
+
+@[simp]
+theorem foldl_empty {α : Type u} {β : Type v} (f_inner : β → α → β) (f_outer : β → β → β)
+    (init_inner init_outer : β) (start stop : Fin empty.size) :
+      (empty : RangeArray α).foldl f_inner f_outer init_inner init_outer start stop = init_outer := by
+  rcases start with ⟨start, hstart⟩
+  rcases stop with ⟨stop, hstop⟩
+  simp at hstart hstop
+  simp [foldl, hstart, hstop]
+
+structure models (RA : RangeArray α) (A : Array (Array α)) : Prop :=
+  (h_outer_size : RA.size = A.size)
+  (h_inner_size : ∀ (i : Fin RA.size), RA.rsize i = Array.size (A.get ⟨i.val, by
+      have := i.isLt; simp [h_outer_size] at this; exact this⟩))
+  (h_data : ∀ (i : Fin RA.size) (j : Fin (RA.rsize i)), RA.get i j = (A.get ⟨i.val, by
+      have := i.isLt; simp [h_outer_size] at this; exact this⟩).get ⟨j.val, by
+        have := j.isLt; simp [h_inner_size] at this; exact this⟩)
+
+instance [ToString α] : ToString (RangeArray α) where
+  toString A := A.foldl (· ++ s!" {·}") (· ++ "\n" ++ ·) "" ""
+
+end RangeArray
+
+open LeanSAT LeanSAT.Model PropFun
+
+abbrev FlatCnf := RangeArray ILit
+
+namespace FlatCnf
+
+open RangeArray
+
+instance : ToString FlatCnf where
+  toString F := F.foldl (· ++ s!" {·}") (· ++ "\n" ++ ·) "" ""
+
+def toPropFun (F : FlatCnf) : PropFun IVar :=
+    F.foldl (· ⊔ ·.toPropFun) (· ⊓ ·) ⊥ ⊤
+      ⟨0, F.h_indexes_size_pos⟩ ⟨F.size - 1, by
+        match hF' : F.size with
+        | 0 =>
+          have hF := F.h_indexes_size_pos
+          simp [hF'] at hF
+        | n + 1 => simp⟩
+
+def backToPropFun (F : FlatCnf) : PropFun IVar :=
+  F.foldl_index (· ⊔ ·.toPropFun) ⊥ ⟨F.size - 1, by
+    match hF' : F.size with
+    | 0 =>
+      have hF := F.h_indexes_size_pos
+      simp [hF'] at hF
+    | n + 1 => simp⟩
+
+@[simp]
+theorem toPropFun_empty : toPropFun (RangeArray.empty : FlatCnf) = ⊤ := by
+  simp [toPropFun]
+
+@[simp]
+theorem backToPropFun_empty : backToPropFun (RangeArray.empty : FlatCnf) = ⊥ := by
+  simp [backToPropFun]
+
+variable (F : FlatCnf) (l : ILit)
+
+@[simp]
+theorem backToPropFun_push : backToPropFun (push F l) = F.backToPropFun ⊔ l.toPropFun := by
+  simp [backToPropFun, push, Id.run]
+  sorry
+  done
+
+end FlatCnf
+
+
+#exit
 def get  (i : Fin A.data.size) : α := A.data.get i
 def get? (i : Nat) : Option α := A.data.get? i
 def get! [Inhabited α] (A : RangeArray α) (i : Nat) : α := A.data.get! i
@@ -227,12 +489,47 @@ def foldrOverIndices {β : Type v} (f : Nat → β → β) (init : β) (A : Rang
 
 /- The goal is to prove that the RangeArray acts like an array of arrays. -/
 
+/-
 section fromArrays
 
-variable (as : Array (Array α))
+variable (as : Array (Array α)) (RA : RangeArray α)
 
 def fromArrays : RangeArray α :=
-  as.foldl (fun A a => (a.foldl (fun A x => A.push x) A).cap) (RangeArray.empty)
+  as.foldl (fun RA a => (a.foldl (fun RA x => RA.push x) RA).cap) (RangeArray.empty)
+
+@[simp]
+theorem fromArrays_empty : (fromArrays (#[] : Array (Array α))) = RangeArray.empty := by
+  simp [fromArrays, empty, foldl]
+
+@[simp]
+theorem fromArrays_nil : (fromArrays ({ data := [] } : Array (Array α))) = RangeArray.empty := by
+  simp [fromArrays, empty, foldl]
+
+@[simp]
+theorem foldlM_eq {α : Type u} {β : Type v} {m : Type v → Type w} [Monad m]
+    (f : β → α → m β) (init : β) (as : Array (Array α))
+      (index : Nat) (h_index : index < as.size) :
+    (fromArrays as).foldlMAtIndex f init index = (as.get ⟨index, h_index⟩).foldlM f init := by
+  have ⟨as⟩ := as
+  rw [foldlMAtIndex]
+  induction' as with A AS ih generalizing index
+  · simp at h_index
+  · match index with
+    | 0 =>
+      simp [fromArrays, Array.foldl_eq_foldl_data]
+      done
+    done
+  done
+  -/
+
+
+
+def toPropFun (A : RangeArray ILit) : PropFun IVar :=
+  Fin.foldl A.numPartitions (fun F index =>
+    A.foldlAtIndex)
+  --sorry
+
+#exit
 
 @[simp] theorem size_fromArrays : (fromArrays as).size = as.size := by sorry
   /-rcases as with ⟨as⟩
