Experiments/ProofChecking/SRParser.lean
@@ -1,0 +1,225 @@
+/-
+
+A parser for the LSR proof format.
+
+Authors: Cayden Codel
+Carnegie Mellon University
+
+-/
+
+import LeanSAT.Solver.Dimacs
+import Experiments.ProofChecking.RangeArray
+import Experiments.ProofChecking.SRChecker
+
+import Std
+
+open Std
+open LeanSAT.Solver.Dimacs
+open LeanSAT LeanSAT.Model ILit
+
+namespace SRParser
+
+open Except
+open SR
+
+structure ArrayParseRes where
+  vars : Nat
+  clauses : ICnf
+
+structure RAPraseRes where
+  vars : Nat
+  formula : FlatCnf
+
+def parseLit (maxVar : Nat) (F : FlatCnf) (s : String) : Except (Except String FlatCnf) FlatCnf := do
+  match s.toInt? with
+  | none => throw (throw s!"Literal is not a number: {s}")
+  | some n =>
+    if hn : n = 0 then
+      throw (return F.cap)
+    else
+      if n.natAbs > maxVar then
+        throw (throw s!"Literal {n} is greater than the maximum variable {maxVar}")
+      else
+        if n < 0 then
+          return F.push ⟨n, hn⟩
+        else
+          return F.push ⟨n, hn⟩
+
+def parseClause (maxVar : Nat) (F : FlatCnf) (s : String) : Except String FlatCnf :=
+  match s.splitOn " " |>.foldlM (parseLit maxVar) F with
+  | ok _ => throw "Zero not encountered on this line"
+  | error e => return ← e
+
+def parseFormula (s : String) : Except String FlatCnf := do
+  let ⟨pLine, clauseLines⟩ ←
+    s.splitOn "\n"
+    |>.filter (fun line => !line.startsWith "c" && line.any (!·.isWhitespace))
+    |>.expectNonempty fun () => "All lines are empty or comments"
+  let (nvars, ncls) ← parseHeader pLine
+  let F ← clauseLines.foldlM (parseClause nvars) RangeArray.empty
+  if RangeArray.caps F != ncls then
+    throw s!"Expected {ncls} clauses, but found {F.size}"
+  else
+    return F
+
+inductive LPRCheckingMode
+| Clause   : LPRCheckingMode
+| Witness  : LPRCheckingMode
+| Reducing : LPRCheckingMode
+| DoneWithLine : LPRCheckingMode
+deriving BEq
+
+inductive SRParsingMode
+| clause
+| witness_tf
+| witness_mapped_ready
+| witness_mapped_halfway : IVar → SRParsingMode
+| up_hints
+| rat_hints : Nat × Array Nat → SRParsingMode
+| done_with_line -- Could be removed, in favor of Except (Except String SRLine), but this is arguably more elegant
+deriving BEq
+
+open SRParsingMode
+
+structure SRDeletionLine where
+  clauses : Array Nat
+
+def parseSRAtom (pivot : Option ILit) (p : SRLine × SRParsingMode) (s : String) : Except String (SRLine × SRParsingMode) :=
+  let ⟨line, mode⟩ := p
+  -- No matter what, the string should be a number, so parse it as an int
+  match s.toInt? with
+  | none => throw s!"Atom {s} didn't parse to a number"
+  | some n =>
+    if hn : n = 0 then
+      match mode with
+      | .clause => return ⟨line, .up_hints⟩
+      | .witness_tf => return ⟨line, .up_hints⟩
+      | .witness_mapped_ready => return ⟨line, .up_hints⟩
+      | .witness_mapped_halfway _ => throw s!"Only got half a substitution mapping when ending a witness"
+      | .up_hints => return ⟨line, .done_with_line⟩
+      | .rat_hints hints => return ⟨{ line with rat_hints := line.rat_hints.push hints }, .done_with_line⟩
+      | .done_with_line => throw s!"Addition line continued after last ending 0"
+    else
+      match mode with
+      | .clause =>
+        match pivot with
+        | none => throw "No pivot provided for the clause"
+        | some pivot =>
+          if n = pivot.val then
+            -- Seeing the pivot again means we're parsing a witness
+            return ⟨line, .witness_tf⟩
+          else
+            -- It's not the pivot (and it's not 0), so add it to the clause
+            return ⟨{ line with clause := line.clause.push ⟨n, hn⟩ }, .clause⟩
+      | .witness_tf =>
+        match pivot with
+        | none => throw "No pivot provided for the witness"
+        | some pivot =>
+          if n = pivot.val then
+            -- Seeing the pivot again means we're parsing the substitution mappings
+            return ⟨line, .witness_mapped_ready⟩
+          else
+            return ⟨{ line with witness_lits := line.witness_lits.push ⟨n, hn⟩ }, .witness_tf⟩
+      | .witness_mapped_ready =>
+        match pivot with
+        | none => throw "No pivot provided for the witness"
+        | some pivot =>
+          if n = pivot.val then
+            throw s!"Saw pivot again in substitution mapping"
+          else
+            if n < 0 then
+              throw s!"First of a substitution mapping must be positive"
+            else
+              return ⟨line, .witness_mapped_halfway ⟨n.natAbs, Int.natAbs_pos.mpr hn⟩⟩
+      | .witness_mapped_halfway v =>
+        return ⟨{line with witness_maps := line.witness_maps.push ⟨v, ⟨n, hn⟩⟩ }, .witness_mapped_ready⟩
+      | .up_hints =>
+        if n < 0 then
+          match pivot with
+          | none => throw "Can't have RAT hints for empty clauses"
+          | _ =>
+            -- This is our first RAT hint - start building it
+            return ⟨line, .rat_hints ⟨n.natAbs - 1, #[]⟩⟩
+        else
+          return ⟨{ line with up_hints := line.up_hints.push (n.natAbs - 1) }, .up_hints⟩
+      | .rat_hints ⟨h, hints⟩ =>
+        if n < 0 then
+          -- This is a new RAT hint - add the old one
+          return ⟨{ line with rat_hints := line.rat_hints.push ⟨h, hints⟩ }, .rat_hints ⟨n.natAbs - 1, #[]⟩⟩
+        else
+          return ⟨line, .rat_hints ⟨h, hints.push (n.natAbs - 1)⟩⟩
+      | .done_with_line => throw s!"Addition line continued after last ending 0"
+
+def parseLSRLine (p : Nat × Array (SRLine ⊕ SRDeletionLine)) (s : String) : Except String (Nat × Array (SRLine ⊕ SRDeletionLine)) :=
+  let ⟨maxId, lines⟩ := p
+  match s.splitOn " " with
+  | [] => throw "Empty line"
+  | [_] => throw s!"Single atom line: {s}, with id {maxId}"
+  | (id :: hd :: tls) =>
+    match hd with
+    | "d" =>
+      -- Check to make sure the maxId is (non-strictly) monotonically increasing
+      match id.toNat? with
+      | none => throw "Line ID is not a number"
+      | some id =>
+        if id < maxId then
+          throw "Deletion line id is not increasing"
+        else
+          match tls.foldlM (fun arr str =>
+            match str.toNat? with
+            | none => throw (throw s!"{str} was not a number")
+            | some 0 => throw (return arr)
+            | some (n + 1) => return arr.push n) #[] with
+          | ok _ => throw "Zero not found on deletion line"
+          | error e => return ⟨max id maxId, lines.push (.inr (SRDeletionLine.mk (← e)))⟩
+    | _ =>
+      -- We have an addition line, so the maxId should strictly increase
+      match id.toNat? with
+      | none => throw "Line ID is not a number"
+      | some id =>
+        if id ≤ maxId then
+          throw "Addition line id is not increasing"
+        else
+          match hd.toInt? with
+          | none => throw "Pivot is not a number"
+          | some n =>
+            let line : SRLine := ⟨#[], #[], #[], #[], #[]⟩
+            if hn : n = 0 then
+              match tls.foldlM (parseSRAtom none) ⟨line, .up_hints⟩ with
+              | error str => throw str
+              | ok ⟨line, mode⟩ =>
+                if mode != .done_with_line then
+                  throw "Addition line for empty clause didn't end with 0"
+                else
+                  return ⟨id, lines.push (.inl line)⟩
+            else
+              match tls.foldlM (parseSRAtom (some ⟨n, hn⟩)) ⟨line, .clause⟩ with
+              | error str => throw str
+              | ok ⟨line, mode⟩ =>
+                if mode != .done_with_line then
+                  throw "Addition line didn't end with 0"
+                else
+                  return ⟨id, lines.push (.inl line)⟩
+
+def parseLSRFile (formulaSize : Nat) (s : String) : Except String (Array (SRLine ⊕ SRDeletionLine)) :=
+  match s.splitOn "\n"
+    |>.filter (fun line => !line.startsWith "c" && line.any (!·.isWhitespace))
+    |>.foldlM parseLSRLine ⟨formulaSize, #[]⟩ with
+  | error e => throw e
+  | ok ⟨_, lines⟩ => return lines
+
+
+end SRParser
+
+def main (args : List String) : IO Unit := do
+  let cnfFile := args[0]!
+  let lsrFile := args[1]!
+  let contents ← IO.FS.withFile cnfFile .read (·.readToEnd)
+  --let res ← fromFileEnc cnfFile
+  let F ← IO.ofExcept <| SRParser.parseFormula contents
+  IO.println s!"Formula has {RangeArray.caps F} clauses"
+
+  let lsrContents ← IO.FS.withFile lsrFile .read (·.readToEnd)
+  let lines ← IO.ofExcept <| SRParser.parseLSRFile (RangeArray.caps F) lsrContents
+  IO.println s!"LSR file has {lines.size} lines"
+  --IO.println s!"{F}"
