lakefile.lean
@@ -16,5 +16,9 @@ lean_lib Experiments {
   globs := #[.submodules `Experiments]
 }
 
+lean_exe «FormulaParser» {
+  root := `Experiments.ProofChecking.SRParser
+}
+
 -- Note: `mathlib` and `std` are obtained transitively so that the versions all match up
 require leancolls from git "https://github.com/JamesGallicchio/LeanColls.git" @ "main"
